Refactor aux functions and wellformedness

src/SchemaAux.v
@@ -20,9 +20,9 @@ Section SchemaAux.
 
   
   (* Schema used as parameter in later functions *) 
-  Implicit Type schema : @schema Name.
+  Variable schema : @schema Name.
 
-  
+  Notation type := (@type Name).
 
   Fixpoint get_first {A} p (lst : seq A) :=
     if lst is hd :: tl then
@@ -32,17 +32,13 @@ Section SchemaAux.
         get_first p tl
     else
       None.
-  
-  (** Get the query root type for the given Schema **)
-  Definition query_root schema : NamedType := schema.(query_type). 
 
   
   (**
    Looks up a name in the given document, returning the type definition if it
    was declared in the document.
    **)
-  Definition lookup_type schema (ty : NamedType)  : option TypeDefinition :=
-    let: (Schema _ tdefs) := schema in
+  Definition lookup_type (ty : NamedType)  : option TypeDefinition :=
     let n_eq nt tdef := match tdef with
                        | ScalarTypeDefinition name =>  nt == name 
                        | ObjectTypeDefinition name _  _ =>  nt == name
@@ -51,190 +47,165 @@ Section SchemaAux.
                        | EnumTypeDefinition name _ =>  nt == name
                        end
     in
-    get_first (n_eq ty) tdefs.
+    get_first (n_eq ty) schema.
     
 
 
   (** Checks whether the given type is defined as a Scalar in the Schema **)
-  Definition is_scalar_type schema (ty : NamedType) : bool :=
-    match (lookup_type schema ty) with
+  Definition is_scalar_type (ty : NamedType) : bool :=
+    match (lookup_type ty) with
     | Some (ScalarTypeDefinition _) => true
     | _ => false
     end.
 
   (** Checks whether the given type is defined as an Object in the Schema **)
-  Equations is_object_type schema (ty : @NamedType Name) : bool :=
-    is_object_type schema ty with (lookup_type schema ty) =>
+  Equations is_object_type (ty : @NamedType Name) : bool :=
+    is_object_type ty with (lookup_type ty) =>
     {
       | Some (ObjectTypeDefinition _ _ _) := true;
       | _ => false
     }.
 
-  Lemma is_object_type_E schema ty :
-    is_object_type schema ty ->
-    exists (t : @NamedType Name) intfs flds, lookup_type schema ty = Some (ObjectTypeDefinition t intfs flds).
+  Lemma is_object_type_E ty :
+    is_object_type ty ->
+    exists (t : @NamedType Name) intfs flds, lookup_type ty = Some (ObjectTypeDefinition t intfs flds).
   Proof.
-    funelim (is_object_type schema ty) => // _.
-      by exists s0; exists l; exists l0.
+    funelim (is_object_type ty) => // _.
+      by exists s0, f, l.
   Qed.
 
   (** Checks whether the given type is defined as an Interface in the Schema **)
-  Equations is_interface_type schema (ty : @NamedType Name) : bool :=
-    is_interface_type schema ty with (lookup_type schema ty) =>
+  Equations is_interface_type (ty : @NamedType Name) : bool :=
+    is_interface_type ty with (lookup_type ty) =>
     {
       | Some (InterfaceTypeDefinition _ _) := true;
       | _ => false
     }.
 
-  Lemma is_interface_type_E schema ty :
-    is_interface_type schema ty <->
-    exists i flds, lookup_type schema ty = Some (InterfaceTypeDefinition i flds).
+  Lemma is_interface_type_E ty :
+    is_interface_type ty <->
+    exists i flds, lookup_type ty = Some (InterfaceTypeDefinition i flds).
   Proof.
     split.
-    funelim (is_interface_type schema ty) => // _.
-      by exists s1; exists l1.
+    funelim (is_interface_type ty) => // _.
+      by exists s1, l0.
     case=> i; case=> flds Hlook.
       by rewrite is_interface_type_equation_1 Hlook.
   Qed.
   
   (** Checks whether the given type is defined as a Union in the Schema **)
-  Equations is_union_type schema (ty : @NamedType Name) : bool :=
-    is_union_type schema ty with (lookup_type schema ty) =>
+  Equations is_union_type (ty : @NamedType Name) : bool :=
+    is_union_type ty with (lookup_type ty) =>
     {
       | Some (UnionTypeDefinition _ _) := true;
       | _ => false
     }.
 
-    Lemma is_union_type_E schema ty:
-      is_union_type schema ty <->
-      exists u mbs, lookup_type schema ty = Some (UnionTypeDefinition u mbs).
+    Lemma is_union_type_E ty:
+      is_union_type ty <->
+      exists u mbs, lookup_type ty = Some (UnionTypeDefinition u mbs).
     Proof.
       split.
-      funelim (is_union_type schema ty) => // _.
-        by exists s2; exists l2.
+      funelim (is_union_type ty) => // _.
+        by exists s2, f0.
       case=> u; case=> mbs Hlook.
       by rewrite is_union_type_equation_1 Hlook.  
   Qed.
   
   (** Checks whether the given type is defined as an Enum in the Schema **)
-  Definition is_enum_type schema (ty : NamedType) : bool :=
-    match (lookup_type schema ty) with
+  Definition is_enum_type (ty : NamedType) : bool :=
+    match (lookup_type ty) with
     | Some (EnumTypeDefinition _ _) => true
     | _ => false
     end.
 
   (** Checks whether the given type is a list type (does not care for the wrapped type) **)
-  Definition is_list_type (ty : @type Name) : bool :=
+  Definition is_list_type (ty : type) : bool :=
     match ty with
     | (ListType ty') => true
     | _ => false
     end.
 
 
-
-  Definition types_names (tys : seq type) : seq Name := map (@name_of_type Name) tys.
-
-  (** Get a type definition's name.
-      Corresponds to the name one gives to an object, interface, etc.
-   **)
-  Definition type_def_name (tdef : TypeDefinition) : Name :=
-    match tdef with 
-    | ScalarTypeDefinition name => name
-    | ObjectTypeDefinition name _ _ => name
-    | InterfaceTypeDefinition name _ => name
-    | UnionTypeDefinition name _ => name
-    | EnumTypeDefinition name _ => name
-    end.
-
-  (** Get type definitions' names *)
-  Definition type_defs_names (tdefs : seq TypeDefinition) : seq Name := map type_def_name tdefs.
-
-  Definition is_named tdef (name : Name) : bool :=
-    match tdef with
-    | ScalarTypeDefinition n => n == name
-    | ObjectTypeDefinition n _ _ => n == name
-    | InterfaceTypeDefinition n _ => n == name
-    | UnionTypeDefinition n _ => n == name
-    | EnumTypeDefinition n _ => n == name
-    end.
-
-  (** Get names from a list of arguments **)
-  Definition arguments_names (args : seq FieldArgumentDefinition) : seq Name :=
-    map (@argname Name) args.
-
- 
-  (** Get list of fields declared in an Object or Interface type definition **)
-  Definition fields schema (ty : NamedType) : list FieldDefinition :=
-    match lookup_type schema ty with
-    | Some (ObjectTypeDefinition _ _ flds) => flds
-    | Some (InterfaceTypeDefinition _ flds) => flds
-    | _ => []
-    end.
+  
+  (** Get all unduplicated argument names from a field **)
+  Definition field_arg_names (fld : FieldDefinition) : {fset Name} := fset [seq arg.(argname) | arg <- fld.(field_args)].
 
 
-  Definition fields_names (flds : seq FieldDefinition) : seq Name := map (@field_name Name) flds.
+  (** Get all field names from a type definition **)
+  Definition tdef_field_names (tdef : @TypeDefinition Name) : {fset Name} := fset [seq fld.(field_name) | fld <- tdef.(tdef_fields)].
 
   
+  (** Get list of fields declared in an Object or Interface type definition **)
+  Definition fields (ty : NamedType) : seq FieldDefinition :=
+    match lookup_type ty with
+    | Some (ObjectTypeDefinition _ _ flds) => flds
+    | Some (InterfaceTypeDefinition _ flds) => flds
+    | _ => [::]
+    end.
+
+
+  (** Get all type definitions' names from a schema **)
+  Definition schema_names : {fset Name} := fset [seq tdef.(tdef_name) | tdef <- schema]. 
+
+
+  (** Check whether a given name is declared in the schema, as a type definition **)
+  Definition is_declared (name : Name) : bool := name \in schema_names.
   
   (**
      Gets the first field definition from a given type that matches the given field name. 
      If the type is not declared in the Schema or the field does not belong to the type, then it returns None.
    **)
-  Definition lookup_field_in_type schema (ty : NamedType) (fname : Name) : option FieldDefinition :=
-    let n_eq nt fld := let: Field name _ _ := fld in nt == name
-    in
-    get_first (n_eq fname) (fields schema ty).
-
+  Definition lookup_field_in_type (ty : NamedType) (fname : Name) : option FieldDefinition :=
+    if lookup_type ty is Some tdef then
+      get_first (fun fld => fld.(field_name) == fname) tdef.(tdef_fields)
+    else
+      None.
 
   (** 
       Gets the type of the first field definition from a given type that matches the given field name. 
       If the type is not declared in the Schema or the field does not belong to the type, then it returns None.
 
    **)
-  Definition lookup_field_type schema (ty : NamedType) (fname : Name)  : option type :=
-    match lookup_field_in_type schema ty fname with
+  Definition lookup_field_type (ty : NamedType) (fname : Name)  : option type :=
+    match lookup_field_in_type ty fname with
     | Some fieldDef => Some (return_type fieldDef) 
     | None => None
     end.
 
 
-  (**
+    (**
      Get the union's types' names.
      If the type is not declared as Union in the Schema, then returns None.
    **)
-  Definition union_members schema (ty : NamedType) : seq NamedType :=
-    match lookup_type schema ty with
+  Definition union_members (ty : NamedType) : {fset NamedType} :=
+    match lookup_type ty with
     | Some (UnionTypeDefinition name mbs) => mbs
-    | _ => []
+    | _ => fset0
     end.
 
 
   (**
      Checks whether the given type declares implementation of another type.
    **)
-  Definition declares_implementation schema (ty ty' : NamedType) : bool :=
-    match lookup_type schema ty with
+  Definition declares_implementation (ty ty' : NamedType) : bool :=
+    match lookup_type ty with
     | Some (ObjectTypeDefinition _ intfs _) => ty' \in intfs
     | _ => false
     end.
 
 
   Definition implements_interface (iname : NamedType) (tdef : @TypeDefinition Name) : bool :=
-    match tdef with
-    | ObjectTypeDefinition _ intfs _ => iname \in intfs
-    | _ => false
-    end.
+    iname \in tdef.(tdef_intfs).
   
   (**
      Gets the first argument definition that matches the given argument name, from the
      given type and field. If the argument is not defined then it returns None.
      If the field is not declared in that type, then it returns None.
    **)
-  Definition lookup_argument_in_type_and_field schema (ty : NamedType) (fname argname : Name) : option FieldArgumentDefinition :=
-    match lookup_field_in_type schema ty fname with
-    | Some (Field fname args _) => let n_eq n arg := let: FieldArgument name _ := arg in n == name
-                                  in
-                                  get_first (n_eq argname) args
+  Definition lookup_argument_in_type_and_field (ty : NamedType) (fname aname : Name) : option FieldArgumentDefinition :=
+    match lookup_field_in_type ty fname with
+    | Some (Field fname args _) => get_first (fun arg => arg.(argname) == aname) args
     | _ => None
     end.
 
@@ -248,33 +219,28 @@ Section SchemaAux.
      3. Union : Possible types are all members of the union.
 
    **)
- (* Definition get_possible_types schema (ty : NamedType) : seq NamedType  :=
-    match lookup_type schema ty with
-    | Some (ObjectTypeDefinition _ _ _) => [:: ty]
-    | Some (InterfaceTypeDefinition iname _) =>
-      (type_defs_names (filter (implements_interface iname) schema.(typeDefinitions)))
-    | Some (UnionTypeDefinition _ mbs) => mbs
-    | _ => [::]
-    end. *)
-
-  Definition get_possible_types schema (ty : NamedType) : {fset NamedType} :=
-    match lookup_type schema ty with
+  Definition get_possible_types (ty : NamedType) : {fset NamedType} :=
+    match lookup_type ty with
     | Some (ObjectTypeDefinition _ _ _) => fset1 ty
     | Some (InterfaceTypeDefinition iname _) =>
-      fset (type_defs_names (filter (implements_interface iname) schema.(typeDefinitions)))
+      let filtered := [seq tdef <- schema | implements_interface iname tdef]
+      in
+      fset [seq tdef.(tdef_name) | tdef <- filtered]
     | Some (UnionTypeDefinition _ mbs) => fset mbs
     | _ => fset0
     end.
   
-  Definition implementation schema (ty : NamedType) : seq NamedType :=
-     match lookup_type schema ty with
+  Definition implementation (ty : NamedType) : seq NamedType :=
+    match lookup_type ty with
     | Some (InterfaceTypeDefinition iname _) =>
-      type_defs_names (filter (implements_interface iname) schema.(typeDefinitions))
+      let filtered := [seq tdef <- schema | implements_interface iname tdef]
+      in
+      fset [seq tdef.(tdef_name) | tdef <- filtered]
     | _ => [::]
     end.
 
-  Lemma declares_in_implementation schema t ty :
-    (declares_implementation schema t ty) <-> (t \in implementation schema ty).
+  Lemma declares_in_implementation t ty :
+    (declares_implementation t ty) <-> (t \in implementation ty).
   Proof.
   Admitted.
   
@@ -299,12 +265,12 @@ Section SchemaAux.
     * move=> [Heq | Hintfs | Hunion].
       rewrite /get_possible_types.
   Qed. *)
-  
-  Lemma in_possible_types_E schema t ty :
-    t \in get_possible_types schema ty ->
+
+  Lemma in_possible_types_E t ty :
+    t \in get_possible_types ty ->
           [\/ t = ty,
-           t \in implementation schema ty |
-           t \in union_members schema ty].
+           t \in implementation ty |
+           t \in union_members ty].
   Proof.
     rewrite /get_possible_types.
     case Hlook : lookup_type => [tdef|] //.
@@ -312,15 +278,17 @@ Section SchemaAux.
     - move=> obj intfs flds Hlook.
         by rewrite in_fset1; move/eqP; constructor 1.
     - move=> intf flds Hlook.
-        by rewrite in_fset /implementation Hlook; constructor 2.
+        by rewrite in_fset /implementation Hlook; constructor 2; rewrite in_fset.
     - move=> un mbs Hlook.
         by rewrite in_fset /union_members Hlook; constructor 3.
   Qed.
+
+
+ 
   
 End SchemaAux.
 
 
-Arguments query_root [Name].
 Arguments lookup_type [Name].
 Arguments is_enum_type [Name].
 
